lean/Nucleus/Nucleus/Hol.lean
@@ -4,6 +4,10 @@ import Nucleus.Hol.Nat
 import Nucleus.Hol.Soundness
 import Nucleus.Hol.Intrinsic
 import Nucleus.Hol.FamilySub
+import Nucleus.Hol.FamilySub.Substitution
+import Nucleus.Hol.FamilySub.Kernel
+import Nucleus.Hol.FamilySub.Product
+import Nucleus.Hol.FamilySub.Coproduct
 
 /-!
 # Signature-parametric HOL
